code/ecdsa/Hacl.Impl.EC.Setup.fst
@@ -419,8 +419,9 @@ let upload_b_constant #c x =
 val uploadBasePoint: #c: curve -> p: point c -> Stack unit 
   (requires fun h -> live h p)
   (ensures fun h0 _ h1 -> 
-    modifies (loc p) h0 h1 /\ point_eval c h1 p /\ (
-    basePoint #c == fromDomainPoint #c #DH (point_as_nat c h1 p)))
+    modifies (loc p) h0 h1 /\ point_eval c h1 p /\ 
+    ~ (isPointAtInfinity (point_as_nat c h1 p)) /\ 
+    basePoint #c == fromDomainPoint #c #DH (point_as_nat c h1 p))
 
 let uploadBasePoint #c p = 
   match c with
